src/parser/FStar.Parser.Const.fst
@@ -554,5 +554,6 @@ let fext_on_dom_g_lid = fext_lid "on_dom_g"
 let sealed_lid      = p2l ["FStar"; "Sealed"; "sealed"]
 let seal_lid        = p2l ["FStar"; "Sealed"; "seal"]
 let unseal_lid      = p2l ["FStar"; "Tactics"; "Builtins"; "unseal"]
+let tref_lid        = p2l ["FStar"; "Tactics"; "Types"; "tref"]
 
 let issue_lid = p2l ["FStar"; "Issue"; "issue"]
